calculate all permutations formula

src/Util/FisherYates/Correctness.dfy
@@ -4,7 +4,6 @@
  *******************************************************************************/
 
 module FisherYates.Correctness {
-  import Permutations
   import Model
   import Rand
   import Uniform
@@ -12,14 +11,45 @@ module FisherYates.Correctness {
   import Independence
   import RealArith
 
-  lemma {:rlimit 1000} {:vcs_split_on_every_assert} CorrectnessFisherYates<T(!new)>(xs: seq<T>, p: seq<T>)
-    requires Permutations.IsPermutationOf(p, xs)
+  /************
+   Definitions
+  ************/
+
+  // Number of permutations of s[i..] == [s[i], s[i+1], ..., s[|s|-1]]
+  function NumberOfPermutationsOf<T(==)>(s: seq<T>, i: nat := 0): (n: nat)
+    requires |s| != 0 ==> i <= |s| - 1
+    decreases |s| - i
+    ensures n != 0
+  {
+    if |s| == 0 || i == |s| - 1 then
+      1
+    else
+      var multiplicity := multiset(s[i..])[s[i]];
+      var length := |s[i..]|;
+      (length / multiplicity) * NumberOfPermutationsOf(s, i+1)
+  }
+
+  /*******
+   Lemmas
+  *******/
+
+  lemma {:axiom} CorrectnessFisherYates<T(!new)>(xs: seq<T>, p: seq<T>)
+    requires multiset(p) == multiset(xs)
     ensures
       var e := iset s | Model.Shuffle(xs)(s).Equals(p);
       && e in Rand.eventSpace
-      && |Permutations.CalculateAllPermutationsOf(xs)| > 0
-      && Rand.prob(e) == 1.0 / (|Permutations.CalculateAllPermutationsOf(xs)| as real)
-  {
+      && Rand.prob(e) == 1.0 / (NumberOfPermutationsOf(xs) as real)
+  /*   {
+      CorrectnessFisherYatesGeneral(xs, p, 0);
+    } */
+
+  /*   lemma {:axiom} CorrectnessFisherYatesGeneral<T(!new)>(xs: seq<T>, p: seq<T>, i: nat)
+      requires multiset(p) == multiset(xs)
+      ensures
+        var e := iset s | Model.Shuffle(xs, i)(s)[i..].Equals(p[i..]);
+        && e in Rand.eventSpace
+        && Rand.prob(e) == 1.0 / (NumberOfPermutationsOf(xs, i) as real) */
+  /* {
     var e := iset s | Model.Shuffle(xs)(s).Equals(p);
     assume {:axiom} e in Rand.eventSpace; // todo later
 
@@ -29,16 +59,16 @@ module FisherYates.Correctness {
         (j: int) requires 0 <= j < |xs| => 
           var zs := Permutations.Swap(xs, 0, j);
           Monad.Map(Model.Shuffle(zs[1..]), (ys: seq<T>) => [zs[0]] + ys);
-
+      var j: int := Permutations.FirstOccurrence(xs, p[0]);
+      var A: iset<int> := iset{j};
+      var B: iset<seq<T>> := iset xs | xs[1..] == p[1..];
+      var E: iset<Rand.Bitstream> := Monad.BitstreamsWithValueIn(f(j), B);
+      var zs := Permutations.Swap(xs, 0, j)[1..];
+      assume {:axiom} false;
       assert Independence.IsIndep(h) by {
         Uniform.Correctness.IntervalSampleIsIndep(0, |xs|);
       }    
-      var j: int := Permutations.FirstOccurrence(xs, p[0]);
-      var A: iset<int> := iset{j};
-      var A2: iset<seq<T>> := iset xs | xs[1..] == p[1..];
-      var E: iset<Rand.Bitstream> := Monad.BitstreamsWithValueIn(f(j), A2);
-      var zs := Permutations.Swap(xs, 0, j)[1..];
-      assert A1: Rand.prob(iset s | s in Monad.BitstreamsWithValueIn(h, A)) == 1.0 / |xs| as real by {
+      assert Eq1: Rand.prob(iset s | s in Monad.BitstreamsWithValueIn(h, A)) == 1.0 / |xs| as real by {
         calc {
           Rand.prob(iset s | s in Monad.BitstreamsWithValueIn(h, A));
           Rand.prob(iset s | Uniform.Model.IntervalSample(0, |xs|)(s).Equals(j));
@@ -46,10 +76,10 @@ module FisherYates.Correctness {
           1.0 / |xs| as real;
         }
       }
-      assert A2: Rand.prob(E) == 1.0 / (|Permutations.CalculateAllPermutationsOf(zs)| as real) by {
+      assert Eq2: Rand.prob(E) == 1.0 / (|Permutations.CalculateAllPermutationsOf(zs)| as real) by {
         calc {
           Rand.prob(E);
-          Rand.prob(Monad.BitstreamsWithValueIn(f(j), A2));
+          Rand.prob(Monad.BitstreamsWithValueIn(f(j), B));
           Rand.prob(iset s | f(j)(s).Result? && f(j)(s).value[1..] == p[1..]);
           Rand.prob(iset s | Model.Shuffle(zs)(s).Equals(p[1..]));
           1.0 / (|Permutations.CalculateAllPermutationsOf(zs)| as real);
@@ -62,7 +92,7 @@ module FisherYates.Correctness {
         Rand.prob(iset s | s in Monad.BitstreamsWithValueIn(h, A) && s in Monad.BitstreamsWithRestIn(h, E));
         { Independence.ResultsIndependent(h, A, E); }
         Rand.prob(iset s | s in Monad.BitstreamsWithValueIn(h, A)) * Rand.prob(E);
-        { reveal A1; reveal A2; }
+        { reveal Eq1; reveal Eq2; }
         (1.0 / |xs| as real) * (1.0 / |Permutations.CalculateAllPermutationsOf(zs)| as real);
         { RealArith.SimplifyFractionsMultiplication(1.0, |xs| as real, 1.0, |Permutations.CalculateAllPermutationsOf(zs)| as real); }
         (1.0 * 1.0) / (|xs| as real * |Permutations.CalculateAllPermutationsOf(zs)| as real);
@@ -74,6 +104,6 @@ module FisherYates.Correctness {
     } else { 
       assume {:axiom} false; // todo later
     }
-  }
+  } */
 
 }
