src/Util/FisherYates/Model.dfy
@@ -5,20 +5,31 @@
 
 module FisherYates.Model {
   import Monad
-  import Permutations
   import Uniform
   import Rand
 
-  opaque ghost function Shuffle<T>(xs: seq<T>, i: nat := 0): Monad.Hurd<seq<T>>
+  ghost function Shuffle<T>(xs: seq<T>, i: nat := 0): Monad.Hurd<seq<T>>
     requires i <= |xs|
     decreases |xs| - i
   {
-    (s: Rand.Bitstream) => 
+    (s: Rand.Bitstream) =>
       if i < |xs| then
         var (j, s) :- Uniform.Model.IntervalSample(i, |xs|)(s);
-        var xs := Permutations.Swap(xs, i, j);
+        var xs := Swap(xs, i, j);
         Shuffle(xs, i + 1)(s)
-      else 
+      else
         Monad.Return(xs)(s)
+  }
+
+  function Swap<T>(s: seq<T>, i: nat, j: nat): (t: seq<T>)
+    requires i <= j
+    requires 0 <= i < |s|
+    requires 0 <= j < |s|
+    ensures |s| == |t|
+  {
+    if i == j then
+      s
+    else
+      s[..i] + [s[j]] + s[i+1..j] + [s[i]] + s[j+1..]
   }
 }
