src/ProbabilisticProgramming/Loops.dfy
@@ -109,7 +109,7 @@ module Loops {
       var reject := (a: A) => !accept(a);
       var body := (a: A) => proposal;
       forall s :: f(s) == proposal(s).Bind(While(reject, body))
-    ensures 
+    ensures
       forall s | f(s).Result? :: accept(f(s).value)
   {
     reveal While();
